   \ \\ [-5mm]
   \begin{enumerate}
      \item $\dfrac23+\dfrac76 =\dfrac46+\dfrac76 =\blue \dfrac{11}6$ \bigskip
      \item $\dfrac67-\dfrac3{14} =\dfrac{12}{14}-\dfrac3{14} =\blue \dfrac9{14}$ \bigskip
      \item $\dfrac{38}{13}-\dfrac3{39} =\dfrac{114}{39}-\dfrac3{39} =\dfrac{111}{39} =\blue \dfrac{37}{13}$ \bigskip
      \item $\dfrac{18}{46}+\dfrac{28}{23} =\dfrac{9}{23}+\dfrac{28}{23} =\blue \dfrac{37}{23}$ \bigskip
      \item $\dfrac83-\dfrac26-\dfrac4{12} =\dfrac{32}{12}-\dfrac{4}{12}-\dfrac{4}{12} =\dfrac{24}{12} =\blue 2$ \bigskip
      \item $\dfrac12+\dfrac34+\dfrac58 =\dfrac48+\dfrac68+\dfrac58 =\blue \dfrac{15}{8}$ \bigskip
      \item $\dfrac34-4-\dfrac5{16} =\dfrac{12}{16}-\dfrac{64}{16}-\dfrac{5}{16} =\blue -\dfrac{57}{16}$ \bigskip
      \item $\dfrac{12}{49}+2-\dfrac97 =\dfrac{12}{49}+\dfrac{98}{49}-\dfrac{63}{49} =\blue \dfrac{47}{49}$
   \end{enumerate}
