\ \\ [-5mm]
   \begin{enumerate}
      \item $5(x-2) =5\times x-5\times2 ={\blue 5x-10}$. \\
         $(-8)\times (k+5) =-8\times k-8\times5 ={\blue -8k-40}$. \\
         $(x+5)(4x-1) + (3x+7)(2x-9) =(4x^2-x+20x-5)+(6x^2-27x+14x-63) ={\blue 10x^2+6x-68}$. \\
         $(5x+3)(x-1) -(7x+9)(2x-5) =(5x^2-5x+3x-3)-(14x^2-35x+18x-45) ={\blue -9x^2+15x+42}$.
      \item $7x + 21 =7\times x+7\times3 ={\blue 7(x+3)}$. \\
         $36+42 a =6\times6+6\times7a ={\blue 6(6+7a)}$. \\
         $6y+7y ={\blue 13y}$. \\
         $\underline{(x+7)}(4x+5) + \underline{(x+7)}(2x-1) =\underline{(x+7)}[(4x+5)+(2x-1)] ={\blue (x+7)(6x+4)}$. \\
         $\underline{(7x-8)}(4x+3)-\underline{(7x-8)}(5x+2) =\underline{(7x-8)}[(4x+3)-(5x+2)] ={\blue (7x-8)(-x+1)}$.
   \end{enumerate}
